examples/l3-machine-code/arm/arm_stepLib.sig
@@ -4,8 +4,8 @@ sig
    val arm_instruction: Term.term list -> string list
    val arm_step: string -> string -> Thm.thm list
    val arm_step_hex: string -> string -> Thm.thm list
-   val decode_arm: Term.term list -> bool list * Term.term -> Thm.thm list
-   val decode_arm_hex: Term.term list -> string -> Thm.thm list
+   val arm_decode: Term.term list -> bool list * Term.term -> Thm.thm list
+   val arm_decode_hex: string -> string -> Thm.thm list
    val hex_to_bits_32: string -> Term.term list
    val list_instructions: unit -> string list
    val print_instructions: unit -> unit
@@ -14,7 +14,7 @@ sig
 
      open arm_stepLib
      val () = print_instructions ()
-     val ev = arm_step "v7"
+     val ev = arm_step "v7,vfp"
      fun pev s = (print (s ^ "\n"); Count.apply ev s);
      val _ = Count.apply (List.map ev) (list_instructions ())
      val _ = Count.apply (List.map (Lib.total pev)) (list_instructions ())
