examples/l3-machine-code/arm_progLib.sig
@@ -4,7 +4,7 @@ sig
 
    val arm_config: string -> unit
    val arm_spec: string -> Thm.thm list
-   val arm_spec_hex: string -> Thm.thm
+   val arm_spec_hex: string -> Thm.thm list
 
    val loadSpecs: Thm.thm -> unit
    val saveSpecs: string -> Thm.thm
